---
layout: post
title: "Optellen"
date: 2024-09-12
---
We start with the set of equations:
<div>\[\begin{aligned}
U_t &= \epsilon^2U_{xx}+f(U,V)\\
V_t &= V_{xx}-f(U,V)
\end{aligned}
\]</div>
By previous analysis, we know that we get a 1 parameter family in $$K$$ of pulses and fronts described by a Hamiltonian system in $$U$$, for which there is a specific $$K^*$$ for which we obtain a front solution. Take this $$K^*$$ and the front $$(U^*,V^*)=(U^*,K^*-\epsilon^2 U^*)$$ that comes with it. We can expand these values and obtain:
<div>\[
\begin{aligned}
K^*&=K^*_0+\epsilon^2K_1^*+\mathcal O(\epsilon^4)\\
U^*&=U^*_0+\epsilon^2U_1^*+\mathcal O(\epsilon^4)\\
V^*&=V^*_0+\epsilon^2V_1^*+\mathcal O(\epsilon^4) = K^*_0+\epsilon^2 K_1^*-\epsilon^2 U_0^*+\mathcal O(\epsilon^4)
\end{aligned}
\]</div>
Let's perturb the system to check stability, take $$\delta$$ smaller than all system scales, and define:
<div>\[\begin{aligned}
U(\xi) &= U^*(\xi)+\delta \exp(\lambda t)u(\xi)\\
V(\xi) &= V^*(\xi)+\delta \exp(\lambda t)v(\xi)
\end{aligned}\]</div>
Inserting this into the PDE and throwing out terms of order $$\delta^2$$, we get the linearized equations:
<div>\[
\begin{aligned}
\lambda u &= \epsilon^2u_{xx}+f_U(U^*,V^*)u+f_V(U^*,V^*)v\\
\lambda v&= v_{xx}-f_U(U^*,V^*)u-f_V(U^*,V^*)v
\end{aligned}
\]</div>
Completely expanded we find (check order error lieve makker):
<div>\[
\begin{aligned}
\epsilon^2 \hat\lambda (u_0+\epsilon^2 u_1) &= \epsilon^2(u_0+\epsilon^2 u_1)_{xx}+[f_U^* +\epsilon^2f_{UU}^* U_1^*+\epsilon^2f_{UV}^* (K_1^*-U_0^*)](u_0+\epsilon^2 u_1)\\
&+[f_V^* +\epsilon^2f_{VU}^* U_1^*+\epsilon^2f_{VU}^* (K^*_1-U_0^*)](v_0+\epsilon^2 v_1+\epsilon^4 v_2)+\mathcal O(\epsilon^6)\\
\epsilon^2 \hat\lambda (v_0+\epsilon^2 v_1)&= (v_0+\epsilon^2 v_1+\epsilon^4 v_2)_{xx}+[-f_U^* -\epsilon^2f_{UU}^* U_1^*-\epsilon^2f_{UV}^* (K_1^*-U_0^*)](u_0+\epsilon^2 u_1)\\
&+[-f_V^* -\epsilon^2f_{VU}^* U_1^*-\epsilon^2f_{VU}^* (K^*_1-U_0^*)](v_0+\epsilon^2 v_1+\epsilon^4 v_2)+\mathcal O(\epsilon^6)\\
\end{aligned}
\]</div>adding these two we get:
<div>\[
\begin{aligned}
\epsilon^2 \hat\lambda (u_0+\epsilon^2 u_1+v_0+\epsilon^2 v_1) &= (\epsilon^2u_0+\epsilon^4 u_1+v_0+\epsilon^2 v_1+\epsilon^4 v_2)_{xx}+O(\epsilon^6)\\
\end{aligned}
\]</div>
and in the fast coordinate:
<div>\[
\begin{aligned}
\epsilon^4\hat\lambda (u_0+v_0) &= (\epsilon^2u_0+\epsilon^4 u_1+v_0+\epsilon^2 v_1+\epsilon^4 v_2)_{\xi\xi}+O(\epsilon^6)\\
\end{aligned}
\]</div>
We can now check the equations of all orders:
<div>\[
\begin{aligned}
O(1):\quad 0 &= (v_0)_{\xi\xi}\\
O(\epsilon^2):\quad0 &= (u_0+ v_1)_{\xi\xi}\\
O(\epsilon^4):\quad \hat\lambda (u_0+v_0) &= ( u_1+ v_2)_{\xi\xi}\\
\end{aligned}
\]</div>
Via Fredholm alternative, and $$O(1)$$ $$u$$ equations, we need $$v_0=0$$. Then this reduces to:
<div>\[
\begin{aligned}
O(1):\quad  v_0&=0\\
O(\epsilon^2):\quad0 &= (u_0+ v_1)_{\xi\xi}\\
O(\epsilon^4):\quad \hat\lambda u_0 &= ( u_1+ v_2)_{\xi\xi}\\
\end{aligned}
\]</div>
Furthermore, we know that $$u_0=U^*_{0,\xi}$$ solves the equation, so we can assume we know $$u_0$$. Then we also know $$v_1$$ (integration constant = 0 because Fredholm?). Unknowns are then $$u_1,v_2$$, which will in essence be the first order correction to the translational mode. The question is if this correction will then push $$\lambda$$ into the positive or negative region. So all that's left is to solve $$u_1$$, then we should find $$v_2$$ by the third equation. 
The equation for $$u_1$$ is the following:
<div>\[
\hat\lambda u_0 = u_{1,\xi\xi}+f_U^* u_1+[ f_{UU}^* U_1^*+f_{UV}^* (K_1^*-U_0^*)]u_0+ v_1f_V^*
\]</div>
In principle, the operator is the same as what we found earlier:
<div>\[
u_1 = \mathcal L^{-1}g(\xi)
\]</div>
Where $$g(\xi)$$ is:
<div>\[

\]</div>




# Equations for $$U_1^*$$ etc
<div>\[
\begin{aligned}
0 &= \epsilon^2U^*_{xx}+f(U^*,V^*)\\
0 &= V^*_{xx}-f(U^*,V^*)
\end{aligned}
\]</div>
We expand with:
<div>\[
\begin{aligned}
K^*&=K^*_0+\epsilon^2K_1^*+\mathcal O(\epsilon^4)\\
U^*&=U^*_0+\epsilon^2U_1^*+\mathcal O(\epsilon^4)\\
V^*&=V^*_0+\epsilon^2V_1^*+\mathcal O(\epsilon^4) = K^*_0+\epsilon^2 K_1^*-\epsilon^2 U_0^*+\mathcal O(\epsilon^4)
\end{aligned}
\]</div>
Then we get:
<div>\[
\begin{aligned}
0 &= \epsilon^2(U^*_0+\epsilon^2U_1^*)_{xx}+f(U^*_0+\epsilon^2U_1^*,K^*_0+\epsilon^2 K_1^*-\epsilon^2 U_0^*)\\
0 &= (K^*_0+\epsilon^2 K_1^*-\epsilon^2 U_0^*)_{xx}-f(U^*_0+\epsilon^2U_1^*,K^*_0+\epsilon^2 K_1^*-\epsilon^2 U_0^*)
\end{aligned}
\]</div>
we can add the equations and obtain:
<div>\[
\begin{aligned}
0 &= \epsilon^2(U^*_0+\epsilon^2U_1^*)_{xx}+(K^*_0+\epsilon^2 K_1^*-\epsilon^2 U_0^*)_{xx}\\
\end{aligned}
\]</div>
In the fast coordinates:
<div>\[
\begin{aligned}
0 &= (U^*_0+\epsilon^2U_1^*)_{\xi\xi}+f(U^*_0+\epsilon^2U_1^*,K^*_0+\epsilon^2 K_1^*-\epsilon^2 U_0^*)\\
0 &= (K^*_0+\epsilon^2 K_1^*-\epsilon^2 U_0^*)_{\xi\xi}-\epsilon^2f(U^*_0+\epsilon^2U_1^*,K^*_0+\epsilon^2 K_1^*-\epsilon^2 U_0^*)
\end{aligned}
\]</div>
expanding:
<div>\[
\begin{aligned}
f(U^*_0+\epsilon^2U_1^*,K^*_0+\epsilon^2 K_1^*-\epsilon^2 U_0^*) = \\
f(U^*_0,K^*_0)+\epsilon^2f_U(U^*_0,K^*_0)U_1^*+\epsilon^2f_V(U^*_0,K^*_0)( K_1^*- U_0^*)
\end{aligned}
\]</div>
collecting powers:
<div>\[
\begin{aligned}
0 &= (U^*_0+\epsilon^2U_1^*)_{\xi\xi}+f(U^*_0,K^*_0)+\epsilon^2f_U(U^*_0,K^*_0)U_1^*+\epsilon^2f_V(U^*_0,K^*_0)( K_1^*- U_0^*)\\
0 &= (K^*_0+\epsilon^2 K_1^*-\epsilon^2 U_0^*)_{\xi\xi}-\epsilon^2f(U^*_0+\epsilon^2U_1^*,K^*_0+\epsilon^2 K_1^*-\epsilon^2 U_0^*)
\end{aligned}
\]</div>
collecting for real (second eqn not important?)
<div>\[
\begin{aligned}
0 &= (U^*_0)_{\xi\xi}+f(U^*_0,K^*_0)\\
0 &= (U_1^*)_{\xi\xi}+f_U(U^*_0,K^*_0)U_1^*+f_V(U^*_0,K^*_0)( K_1^*- U_0^*)\\
\end{aligned}
\]</div>
Fredholm tells us:
<div>\[
K_1^*  = \frac{\int U^*_0 U^*_{0,\xi} f_V^*}{\int U^*_{0,\xi} f_V^*}
\]</div>

Let's take the derivative of the second equation:
<div>\[
\begin{aligned}
0 &= \partial_\xi(U_1^*)_{\xi\xi} \\
&+\partial_\xi (f_U(U^*_0,K^*_0)U_1^*)\\
&+\partial_\xi(f_V(U^*_0,K^*_0)( K_1^*- U_0^*))\\
&= (U_1^*)_{\xi\xi\xi} \\
&+ f_{UU}(U^*_0,K^*_0)U^*_{0,\xi}U_1^*+f_U(U^*_0,K^*_0)U_{1,\xi}^*\\
&+f_{UV}(U^*_0,K^*_0)U^*_{0,\xi}( K_1^*- U_0^*)+f_V(U^*_0,K^*_0)( - U_{0,\xi}^*)\\
\end{aligned}
\]</div>
Now we look at our original equation for $$u_1$$:
<div>\[
\hat\lambda u_0 = u_{1,\xi\xi}+f_U^* u_1+[ f_{UU}^* U_1^*+f_{UV}^* (K_1^*-U_0^*)]u_0+ v_1f_V^*
\]</div>
and we recognize a lot of terms. Let's write our derivative-equation as follows:
<div>\[
\begin{aligned}
0 &= (U_1^*)_{\xi\xi\xi}+f_U^*U_{1,\xi}^* + [f_{UU}^* U_1^*+f_{UV}^*( K_1^*- U_0^*)-f_V^*] u_0\\
\end{aligned}
\]</div>
Finally, note that $$v_1=-u_0$$ as we found earlier. Then we can replace a lot of terms and end up with:
<div>\[
\hat\lambda u_0 = u_{1,\xi\xi}+f_U^* u_1-[U_{1,\xi\xi\xi}^*+f_U^*U_{1,\xi}^*]
\]</div>
This seems nice, we got rid of the annoying second derivatives and we don't need $$K_1$$ anymore. However, we are now stuck with $$U_1$$. 
So, let's use the Fredholm alternative to find that solutions should satisfy:
<div>\[
\langle \hat\lambda u_0 +U_{1,\xi\xi\xi}^*+f_U^*U_{1,\xi}^*,u_0\rangle = 0
\]</div>
Since $$u_0$$ goes to zero exponentially, we can maybe use partial integration to find some relations. 
Something else we could do is fill our result into the equation for $$\Delta v_\xi$$ [Netjes order nu=2](../optellen/) and we get:
(does this integral converge? can i replace with over entire R?)
<div>\[
\begin{aligned}
\Delta_{fast} v_{\xi}^*&=\epsilon^4\int_\mathbb R [\hat\lambda u_0-u_{1,\xi\xi}]d\xi+O(\epsilon^6)
\end{aligned}
\]</div>
Then we find after filling in:
<div>\[
\begin{aligned}
\Delta_{fast} v_{\xi}^*&=\epsilon^4\int_\mathbb R [\hat\lambda f_U^* u_1-[U_{1,\xi\xi\xi}^*+f_U^*U_{1,\xi}^*]]d\xi+O(\epsilon^6)
\end{aligned}
\]</div>
The integral over $$U^*_{1,\xi\xi\xi}$$ will be zero, by the boundary conditions, so we're left with:
<div>\[
\begin{aligned}
\Delta_{fast} v_{\xi}^*&=\epsilon^4\int_\mathbb R [\hat\lambda f_U^* u_1-f_U^*U_{1,\xi}^*]d\xi+O(\epsilon^6)
\end{aligned}
\]</div>


oke maar waarom doe ik moeilijk, kan niet gewoon $$\Delta_{fast}(v+u)_\xi$$ gematched worden? [sprong som](../optellen/) 

