---
layout: post
title: "Nu is twee!"
date: 2024-10-02
---
<style>
.math-container {
    max-width: 100%; /* Set a maximum width to prevent it from expanding the page */
    overflow-x: auto; /* Enable horizontal scrolling */
    white-space: nowrap; /* Prevent the text from wrapping */
}
</style>

## Nu order 2 Slow

We now look at the slow system, where:
<div class="math-container">\[
\begin{aligned}
\hat\lambda \epsilon^2 \hat u =\epsilon^2 \hat u_{xx}+f_u^*(u^*_0,K_0^*)\hat u+f_v^*(u^*_0,K_0^*)\hat v \\
\hat\lambda \epsilon^{2} \hat v = \hat v_{xx}- f_u^*(u^*_0,K_0^*)\hat u- f_v^*(u^*_0,K_0^*)\hat v 
\end{aligned}
\]</div>
We find that:
Well we require the orders to match so let's substitute $$\hat u=\epsilon^2 \hat{\hat u}$$ (why u?? I guess to match $$\hat v$$) and $$\hat v=\epsilon^2 \hat{\hat v}$$. This doesn't really change the equations much:
<div class="math-container">\[
\begin{aligned}
\hat\lambda \epsilon^2 \hat{\hat u} =\epsilon^2 \hat{\hat u}_{xx}+f_u^*(u^*_0,K_0^*)\hat{\hat u}+f_v^*(u^*_0,K_0^*)\hat{\hat v} \\
\hat\lambda \epsilon^{2} \hat{\hat v} = \hat{\hat v}_{xx}- f_u^*(u^*_0,K_0^*)\hat{\hat u}- f_v^*(u^*_0,K_0^*)\hat{\hat v }
\end{aligned}
\]</div>
Now we find:
<div class="math-container">\[
\hat{\hat u} =- \frac{f_v^*}{f_u^*}\hat{\hat v}+\mathcal O(\epsilon^2)
\]</div>
Because of the constant coefficients, we also get $$\hat{\hat u}_{xx}= - \frac{f_v^*}{f_u^*}\hat{\hat v}_{xx}$$ (is this true? can't higher order terms have $$O(\epsilon^-1)$$ derivatives or something like that?)
Then we also find by adding the two equations:
<div class="math-container">\[
\hat{\hat v}_{xx} =\hat\lambda \epsilon^2(\hat{\hat u}+\hat{\hat v})-\epsilon^2 \hat u_{xx}=\hat\lambda\epsilon^2\frac{f_u^*-f_v^*}{f_u}\hat{\hat v^*}+ \epsilon^2\frac{f_v^*}{f_u^*}\hat{\hat v}_{xx}+\mathcal O(\epsilon^4)
\]</div>
So we get:
<div class="math-container">\[
\hat{\hat v}_{xx}\left(1+\epsilon^2\frac{f_v^*}{f_u^*}\right) =\hat\lambda\epsilon^2\frac{f_u^*-f_v^*}{f_u}\hat{\hat v^*}+\mathcal O(\epsilon^4)
\]</div>
Now we can just divide by this new term, and get the same expression as for $$2<2$$:
<div class="math-container">\[
\hat{\hat v}_{xx} =\hat\lambda\epsilon^2\frac{f_u^*-f_v^*}{f_u}\hat{\hat v^*}+\mathcal O(\epsilon^4)
\]</div>


#### Nu order 2 fast
<div class="math-container">\[\begin{aligned}
\hat\lambda \epsilon^2 \hat u = \hat u_{\xi\xi}+f_u^*(u^*_0,K_0^*)\hat u+f_v^*(u^*_0,K_0^*)\hat v \\
\hat\lambda \epsilon^{2+2} \hat v = \hat v_{\xi\xi}-\epsilon^2 f_u^*(u^*_0,K_0^*)\hat u-\epsilon^2 f_v^*(u^*_0,K_0^*)\hat v 
\end{aligned}\]</div>
So: $$\hat v=\hat K+\mathcal O(\epsilon^2)$$
Then we get the following system:
<div class="math-container">\[
\hat\lambda \epsilon^2 \hat u = \hat u_{\xi\xi}+f_u^*(u^*_0,K_0^*)\hat u+f_v^*(u^*_0,K_0^*)\hat K+\mathcal O(\epsilon^2) \\
\]</div>
We expand $$\hat u$$ as: 
<div class="math-container">\[\hat u=\hat u_0+\epsilon^2\hat u_1\]</div>
and $$\hat K$$ as $$\hat K = \epsilon^2 \hat{\hat K}$$, order 1 is not possible because of the solvability criterion (Appendix). 
And obtain at leading order:
<div class="math-container">\[
\hat u_{0,\xi\xi}+f_u^*(u_0^*,K_0^*)\hat u_0=0
\]</div>
Which we recognize as the homogeneous fast reduced problem, to which $$Au_{0,\xi}^*$$ is the solution. For simplicity we set $$A=1$$ so we get $$\hat u= u^*_{0,\xi}+\epsilon^2\hat u_1$$ So we get at order $$\epsilon^2$$:
<div class="math-container">\[
\hat\lambda u^*_{0,\xi} = \hat u_{1,\xi\xi}+f_u^*(u^*_0,K_0^*)\hat u_1+f_v^*(u^*_0,K_0^*)\hat{\hat K}+\mathcal O(\epsilon^{2}) \\
\]</div>
Which is a homogeneous SL problem with again the same operator $$\mathcal L=\partial_{\xi\xi}+f_u^*(u_0^*,K_0^*)$$. The Fredholm alternative tells us that this equations has solutions which obey:
<div class="math-container">\[
\langle u_{0,\xi}^*, \hat\lambda  u^*_{0,\xi} -f_v^*(u^*_0,K_0^*)\hat{\hat K} \rangle =0
\]</div>
Which gives:
<div class="math-container">\[
\hat{\hat K} = \hat\lambda \frac{\int_I (u_{0,\xi}^*(\xi))^2d\xi}{\int_I f_v^*(u_0^*(\xi),K_0^*)u_{0,\xi}^*(\xi)d\xi}
\]</div>
Since $$u_{0,\xi}^*(\xi)$$ decays exponentially on both sides, the integrals converge and can be replaced by integrals over the entirety of $$\mathbb R$$. 


### Andere techniek voor fast jump? :)

<div class="math-container">\[
\begin{aligned}
\hat\lambda \epsilon^2 \hat u = \hat u_{\xi\xi}+f_u^*(u^*_0,K_0^*)\hat u+\epsilon^{2}f_v^*(u^*_0,K_0^*)\hat{\hat v} \\
\hat\lambda \epsilon^{4} \hat{\hat v} = \epsilon^0 \hat{\hat v}_{\xi\xi}-\epsilon^0 f_u^*(u^*_0,K_0^*)\hat u- \epsilon^{2} f_v^*(u^*_0,K_0^*)\hat{\hat v }
\end{aligned}
\]</div>
Again our favorite trick: we add the equations and get:
<div class="math-container">\[
\begin{aligned}
\hat\lambda \epsilon^2 \hat u +\hat\lambda \epsilon^{4} \hat{\hat v}= \hat u_{\xi\xi}+\epsilon^0 \hat{\hat v}_{\xi\xi}\end{aligned}
\]</div>
We expand $$\hat u$$ and find:
<div class="math-container">\[
\begin{aligned}
\hat\lambda \epsilon^2 (u_{0,\xi}^*+\epsilon^2\hat u_1) +\hat\lambda \epsilon^{4} \hat{\hat v}= (u_{0,\xi}^*+\epsilon^2\hat u_1)_{\xi\xi}+\epsilon^0 \hat{\hat v}_{\xi\xi}\end{aligned}
\]</div>
Integrating this equation, and using the fact that $$u_{0,\xi}^0$$ is a heteroclinic orbit, hence the derivatives go to zero for $$\xi\to\pm \infty$$, we find:
<div class="math-container">\[
\Delta_{fast} \hat{\hat v}_\xi=\begin{aligned}
\int\hat{\hat v}_{\xi\xi}d\xi=\epsilon^2\int \hat\lambda  u_{0,\xi}^*- \hat u_{1,\xi\xi}d\xi+\mathcal O(\epsilon^4)
\end{aligned}
\]</div>
Note how the integral over the correction might have something to do with the interaction term! The difference in derivatives will be matched to $$\lambda$$, hence (possibly) connecting to the velocity of the wave too!

From [Arjen Notes (my interpretation)]({% link _posts/2024-09-12-arjen-notes-(my-interpretation).md %}) we know that:
<div class="math-container">\[
\hat\lambda u^*_{0,\xi} = \hat u_{1,\xi\xi}+f_u^*(u^*_0,K_0^*)\hat u_1+f_v^*(u^*_0,K_0^*)\hat{\hat K}+\mathcal O(\epsilon^{2}+\epsilon^{2\nu}) 
\]</div>
As the order $$\epsilon^2$$ equation for $$u$$. Solving for $$\hat u_1$$ and inserting in the equation above then yields:
<div class="math-container">\[
\begin{aligned}
\Delta_{fast} \hat{\hat v}_\xi=\epsilon^2\int f_u^*(u^*_0,K_0^*)\hat u_1+f_v^*(u^*_0,K_0^*)\hat{\hat K}d\xi+\mathcal O(\epsilon^4)
\end{aligned}
\]</div>
We get an integral condition on the fast jump, which we match to the square root business we found earlier. 

We get the same equation as Arjen, except the lambda term, but I think he forgot an $$\epsilon^\nu$$ there. :)



Probleem: integraal convergeert over het algemeen niet? :((
