---
layout: post
title: "Nu is twee!"
date: 2024-06-20
---

## Nu order 2 Slow

We now look at the slow system, where:
<div>\[
\begin{aligned}
\hat\lambda \epsilon^2 \hat u =\epsilon^2 \hat u_{xx}+f_u^*(u^*_0,K_0^*)\hat u+f_v^*(u^*_0,K_0^*)\hat v \\
\hat\lambda \epsilon^{2} \hat v = \hat v_{xx}- f_u^*(u^*_0,K_0^*)\hat u- f_v^*(u^*_0,K_0^*)\hat v 
\end{aligned}
\]</div>
We find that:
Well we require the orders to match so let's substitute $$\hat u=\epsilon^2 \hat{\hat u}$$ (why u?? I guess to match $$\hat v$$) and $$\hat v=\epsilon^2 \hat{\hat v}$$. This doesn't really change the equations much:
<div>\[
\begin{aligned}
\hat\lambda \epsilon^2 \hat{\hat u} =\epsilon^2 \hat{\hat u}_{xx}+f_u^*(u^*_0,K_0^*)\hat{\hat u}+f_v^*(u^*_0,K_0^*)\hat{\hat v} \\
\hat\lambda \epsilon^{2} \hat{\hat v} = \hat{\hat v}_{xx}- f_u^*(u^*_0,K_0^*)\hat{\hat u}- f_v^*(u^*_0,K_0^*)\hat{\hat v }
\end{aligned}
\]</div>
Now we find:
<div>\[
\hat{\hat u} =- \frac{f_v^*}{f_u^*}\hat{\hat v}+\mathcal O(\epsilon^2)
\]</div>
Because of the constant coefficients, we also get $$\hat{\hat u}_{xx}= - \frac{f_v^*}{f_u^*}\hat{\hat v}_{xx}$$ (is this true? can't higher order terms have $$O(\epsilon^-1)$$ derivatives or something like that?)
Then we also find by adding the two equations:
<div>\[
\hat{\hat v}_{xx} =\hat\lambda \epsilon^2(\hat{\hat u}+\hat{\hat v})-\epsilon^2 \hat u_{xx}=\hat\lambda\epsilon^2\frac{f_u^*-f_v^*}{f_u}\hat{\hat v^*}+ \epsilon^2\frac{f_v^*}{f_u^*}\hat{\hat v}_{xx}+\mathcal O(\epsilon^4)
\]</div>
So we get:
<div>\[
\hat{\hat v}_{xx}\left(1+\epsilon^2\frac{f_v^*}{f_u^*}\right) =\hat\lambda\epsilon^2\frac{f_u^*-f_v^*}{f_u}\hat{\hat v^*}+\mathcal O(\epsilon^4)
\]</div>
Now we can just divide by this new term, and get the same expression as for $$2<2$$:
<div>\[
\hat{\hat v}_{xx} =\hat\lambda\epsilon^2\frac{f_u^*-f_v^*}{f_u}\hat{\hat v^*}+\mathcal O(\epsilon^4)
\]</div>


#### Nu order 2 fast
<div>\[\begin{aligned}
\hat\lambda \epsilon^2 \hat u = \hat u_{\xi\xi}+f_u^*(u^*_0,K_0^*)\hat u+f_v^*(u^*_0,K_0^*)\hat v \\
\hat\lambda \epsilon^{2+2} \hat v = \hat v_{\xi\xi}-\epsilon^2 f_u^*(u^*_0,K_0^*)\hat u-\epsilon^2 f_v^*(u^*_0,K_0^*)\hat v 
\end{aligned}\]</div>
So: $$\hat v=\hat K+\mathcal O(\epsilon^2)$$
Then we get the following system:
<div>\[
\hat\lambda \epsilon^2 \hat u = \hat u_{\xi\xi}+f_u^*(u^*_0,K_0^*)\hat u+f_v^*(u^*_0,K_0^*)\hat K+\mathcal O(\epsilon^2) \\
\]</div>
We expand $$\hat u$$ as: 
<div>\[\hat u=\hat u_0+\epsilon^2\hat u_1\]</div>
and $$\hat K$$ as $$\hat K = \epsilon^2 \hat{\hat K}$$, order 1 is not possible because of the solvability criterion (Appendix). 
And obtain at leading order:
<div>\[
\hat u_{0,\xi\xi}+f_u^*(u_0^*,K_0^*)\hat u_0=0
\]</div>
Which we recognize as the homogeneous fast reduced problem, to which $$Au_{0,\xi}^*$$ is the solution. For simplicity we set $$A=1$$ so we get $$\hat u= u^*_{0,\xi}+\epsilon^2\hat u_1$$ So we get at order $$\epsilon^2$$:
<div>\[
\hat\lambda u^*_{0,\xi} = \hat u_{1,\xi\xi}+f_u^*(u^*_0,K_0^*)\hat u_1+f_v^*(u^*_0,K_0^*)\hat{\hat K}+\mathcal O(\epsilon^{2}) \\
\]</div>
Which is a homogeneous SL problem with again the same operator $$\mathcal L=\partial_{\xi\xi}+f_u^*(u_0^*,K_0^*)$$. The Fredholm alternative tells us that this equations has solutions which obey:
<div>\[
\langle u_{0,\xi}^*, \hat\lambda  u^*_{0,\xi} -f_v^*(u^*_0,K_0^*)\hat{\hat K} \rangle =0
\]</div>
Which gives:
<div>\[
\hat{\hat K} = \hat\lambda \frac{\int_I (u_{0,\xi}^*(\xi))^2d\xi}{\int_I f_v^*(u_0^*(\xi),K_0^*)u_{0,\xi}^*(\xi)d\xi}
\]</div>
Since $$u_{0,\xi}^*(\xi)$$ decays exponentially on both sides, the integrals converge and can be replaced by integrals over the entirety of $$\mathbb R$$. 


### Andere techniek voor fast jump? :)

<div>\[
\begin{aligned}
\hat\lambda \epsilon^2 \hat u = \hat u_{\xi\xi}+f_u^*(u^*_0,K_0^*)\hat u+\epsilon^{2}f_v^*(u^*_0,K_0^*)\hat{\hat v} \\
\hat\lambda \epsilon^{4} \hat{\hat v} = \epsilon^0 \hat{\hat v}_{\xi\xi}-\epsilon^0 f_u^*(u^*_0,K_0^*)\hat u- \epsilon^{2} f_v^*(u^*_0,K_0^*)\hat{\hat v }
\end{aligned}
\]</div>
Again our favorite trick: we add the equations and get:
<div>\[
\begin{aligned}
\hat\lambda \epsilon^2 \hat u +\hat\lambda \epsilon^{4} \hat{\hat v}= \hat u_{\xi\xi}+\epsilon^0 \hat{\hat v}_{\xi\xi}\end{aligned}
\]</div>
We expand $$\hat u$$ and find:
<div>\[
\begin{aligned}
\hat\lambda \epsilon^2 (u_{0,\xi}^*+\epsilon^2\hat u_1) +\hat\lambda \epsilon^{4} \hat{\hat v}= (u_{0,\xi}^*+\epsilon^2\hat u_1)_{\xi\xi}+\epsilon^0 \hat{\hat v}_{\xi\xi}\end{aligned}
\]</div>
Integrating this equation, and using the fact that $$u_{0,\xi}^0$$ is a heteroclinic orbit, hence the derivatives go to zero for $$\xi\to\pm \infty$$, we find:
<div>\[
\Delta_{fast} \hat{\hat v}_\xi=\begin{aligned}
\int\hat{\hat v}_{\xi\xi}d\xi=\epsilon^2\int \hat\lambda  u_{0,\xi}^*- \hat u_{1,\xi\xi}d\xi+\mathcal O(\epsilon^4)
\end{aligned}
\]</div>
Note how the integral over the correction might have something to do with the interaction term! The difference in derivatives will be matched to $$\lambda$$, hence (possibly) connecting to the velocity of the wave too!

From [Arjen Notes (my interpretation)#Fast linearized system](../nu-is-twee!/) we know that:
<div>\[
\hat\lambda u^*_{0,\xi} = \hat u_{1,\xi\xi}+f_u^*(u^*_0,K_0^*)\hat u_1+f_v^*(u^*_0,K_0^*)\hat{\hat K}+\mathcal O(\epsilon^{2}+\epsilon^{2\nu}) 
\]</div>
As the order $$\epsilon^2$$ equation for $$u$$. Solving for $$\hat u_1$$ and inserting in the equation above then yields:
<div>\[
\begin{aligned}
\Delta_{fast} \hat{\hat v}_\xi=\epsilon^2\int f_u^*(u^*_0,K_0^*)\hat u_1+f_v^*(u^*_0,K_0^*)\hat{\hat K}d\xi+\mathcal O(\epsilon^4)
\end{aligned}
\]</div>
We get an integral condition on the fast jump, which we match to the square root business we found earlier. [#Nu order 2](../nu-is-twee!/)

We get the same equation as Arjen, except the lambda term, but I think he forgot an $$\epsilon^\nu$$ there. :)



Probleem: integraal convergeert over het algemeen niet? :((
