---
layout: post
title: "Problem"
date: 2024-06-24
---

<style>
.math-container {
    max-width: 100%;
    overflow-x: auto;
    white-space: nowrap;
}
</style>

# Stability next order without $$\hat v=\epsilon^2 \hat{\hat v}$$ 
We set $$\lambda = \epsilon^2 \hat\lambda$$ 
<div class="math-container">\[
\begin{aligned}
u = u^*+\delta \hat u\exp(\lambda t)\\
v = v^*+\delta v\exp(\lambda t) 
\end{aligned}
\]</div>
<div class="math-container">\[\begin{aligned}
\epsilon^2 \hat\lambda \hat u&=\hat u_{\xi\xi}+f_u(u^*,v^*)\hat u+f_v(u^*,v^*)\hat v\\
\epsilon^4\hat\lambda \hat v&=\hat v_{\xi\xi}-\epsilon^2f_u(u^*,v^*)\hat u-\epsilon^2f_v(u^*,v^*)\hat v
\end{aligned}\]</div>
Using our expansions: 
<div class="math-container">\[\begin{aligned}
u^*&=u^*_0+\epsilon^2u_1^* \\ 
v^*&=K^*-\epsilon^2 u^* = K_0^*+\epsilon^2 (K_1^* -u^*_0)\\
\hat u&=\hat u_0+\epsilon^2\hat u_1\\
\hat v&=\hat v_0+\epsilon^2\hat v_1
\end{aligned}\]</div>
we get:
<div class="math-container">\[
\begin{aligned}
0&=\hat u_{0,\xi\xi}+f_u(u^*_0,v^*_0)\hat u_0+f_v(u^*_0,v^*_0)\hat v_0\\
0&=\hat v_{0,\xi\xi}
\end{aligned}
\]</div>
at leading order and:
<div class="math-container">\[
\begin{aligned}
\epsilon^2 \hat\lambda (\hat u_0+\epsilon^2\hat u_1)&=(\hat u_0+\epsilon^2\hat u_1)_{\xi\xi}+f_u(u^*,v^*)(\hat u_0+\epsilon^2\hat u_1)+f_v(u^*,v^*)(\hat v_0+\epsilon^2\hat v_1)\\
\epsilon^4\hat\lambda (\hat v_0+\epsilon^2\hat v_1)&=(\hat v_0+\epsilon^2\hat v_1)_{\xi\xi}-\epsilon^2f_u(u^*,v^*)(\hat u_0+\epsilon^2\hat u_1)-\epsilon^2f_v(u^*,v^*)(\hat v_0+\epsilon^2\hat v_1)
\end{aligned}
\]</div>
expanding $$f$$ too and tossing terms of order $$4$$:
<div class="math-container">\[
\begin{aligned}
\epsilon^2 \hat\lambda \hat u_0&=(\hat u_0+\epsilon^2\hat u_1)_{\xi\xi}+(f_{u}(u_0^*,K_0^*)+\epsilon^2(f_{uu}(u_0^*,K_0^*)u_1^* \\&+f_{uv}(u_0^*,K_0^*)(K_1^* -u^*_0)))(\hat u_0+\epsilon^2\hat u_1)+(f_{v}(u_0^*,K_0^*)+\epsilon^2(f_{vu}(u_0^*,K_0^*)u_1^* \\&+f_{vv}(u_0^*,K_0^*)(K_1^* -u^*_0)))(\hat v_0+\epsilon^2\hat v_1)\\
0&=(\hat v_0+\epsilon^2\hat v_1)_{\xi\xi}-\epsilon^2f_u(u^*_0,v^*_0)\hat u_0-\epsilon^2f_v(u^*_0,v^*_0)\hat v_0
\end{aligned}
\]</div>
At order 2 we get:
<div class="math-container">\[
\begin{aligned}
\hat\lambda \hat u_0&=\hat u_{1,\xi\xi}+f_{u}(u_0^*,K_0^*)\hat u_1+(f_{uu}(u_0^*,K_0^*)u_1^* +f_{uv}(u_0^*,K_0^*)(K_1^* -u^*_0))\hat u_0\\&+f_{v}(u_0^*,K_0^*)\hat v_1+(f_{vu}(u_0^*,K_0^*)u_1^* +f_{vv}(u_0^*,K_0^*)(K_1^* -u^*_0))\hat v_0\\
0&=\hat v_{1,\xi\xi}-f_u(u^*_0,v^*_0)\hat u_0-f_v(u^*_0,v^*_0)\hat v_0
\end{aligned}
\]</div>
Since $$\hat u_1$$ doesn't influence $$\hat v_1$$, we can integrate twice to solve $$\hat v_1$$. Then the top term is again a inhomogeneous SL problem:
<div class="math-container">\[
g(\xi)=\hat u_{1,\xi\xi}+f_{u}(u_0^*,K_0^*)\hat u_1
\]</div>
Where $$g$$ captures the horror that $$\nu=2$$ created...
Look at the problem here, the term $$f_v$$ in the $$v$$-equation makes the problem non-solvable since in general $$\int f_v \hat v_0\not=0$$, hence we set $$\hat v= \epsilon^2 \hat{\hat v}$$. Then all our troubles become slightly less problematic. 


Take $$i\in\{u,v\}$$ then:
<div class="math-container">\[\begin{aligned}
f_i &= f_i(u_0^*+\epsilon^2 u_1^*,K_0^*+\epsilon^2 (K_1^* -u^*_0))\\
&= f_{i}(u_0^*,K_0^*)+\epsilon^2(f_{iu}(u_0^*,K_0^*)u_1^* +f_{iv}(u_0^*,K_0^*)(K_1^* -u^*_0))
\end{aligned}\]</div>


[View Raw Markdown](/assets/md/Problem.md)
