The linear stability problem can be written as:
$$
\begin{aligned}
\lambda u=\epsilon^2u_{xx}+f_U(\bar U,\bar V)u+f_V(\bar U,\bar V)v\\
\lambda v=v_{xx}-f_U(\bar U,\bar V)u-f_V(\bar U,\bar V)v
\end{aligned}
$$
Or in matrix form:
$$
\lambda \begin{pmatrix}u\\v\end{pmatrix}=\left(\begin{pmatrix}\epsilon^2\partial_{xx}&0\\0&\partial_{xx}\end{pmatrix}+\begin{pmatrix}f_U(\bar U,\bar V)&f_V(\bar U,\bar V)\\ -f_U(\bar U,\bar V)&-f_V(\bar U,\bar V)\end{pmatrix}\right)\begin{pmatrix}u\\v\end{pmatrix}
$$
Or the shorthand, using $p=\begin{pmatrix}u\\v\end{pmatrix}$, $D=\begin{pmatrix}\epsilon^2\partial_{xx}&0\\0&\partial_{xx}\end{pmatrix}$ and $A(x)=\begin{pmatrix}f_U(\bar U,\bar V)&f_V(\bar U,\bar V)\\ -f_U(\bar U,\bar V)&-f_V(\bar U,\bar V)\end{pmatrix}$, we can write it as:
$$
L(x)p=(A(x)+D)p = \lambda p
$$
Now the question becomes, is $L(x)$ self-adjoint? Well we check using the definition:
$$\begin{aligned}
\langle g,Lh\rangle&=
\int g(x)\cdot L(x)h(x)dx\\
&=\int g(x)\cdot A(x)h(x)dx +\int g(x)\cdot Dh(x)dx 
\end{aligned}$$
We can partially integrate twice, use zero-flux BC's and get:
$$\begin{aligned}
&\int g(x)\cdot A(x)h(x)dx +\int g(x)\cdot Dh(x)dx \\
=&\int g(x)\cdot A(x)h(x)dx +\int Dg(x)\cdot h(x)dx
\end{aligned}
$$
But $A$ is not selfadjoint :(

