$$
\mathcal L-\mathcal L_\infty
$$
$$
\mathcal L = \begin{pmatrix}\partial_{\xi\xi}+f^*_U&f_V^* \\ -\epsilon^2 f^*_U&\partial_{\xi\xi}-\epsilon^2 f_V^* \end{pmatrix} 
$$
Dus:
$$
\mathcal L-\mathcal L_\infty = \begin{pmatrix}f^*_U(x)-&f_V^*(x) \\ -f^*_U(x)&f_V^*- f_V^*(x) \end{pmatrix} 
$$


$$
\mathcal L-\mathcal L_\infty = \begin{pmatrix}a(x)-a_\pm&b(x)-b_\pm \\ -a(x)+a_\pm&-b(x)+b_\pm \end{pmatrix} 
$$
$$
(\mathcal L-\mathcal L_\infty)(\mathcal L_\infty-\lambda)^{-1}(u,v) = 
$$


$$
\|(\mathcal L_\infty-\lambda)^{-1}\| \leq C(\lambda)\|f\|
$$
Take weakest decay in $\mathcal L-\mathcal L_\infty$, call it $\alpha$, then:
$$
\|(\mathcal L-\mathcal L_\infty)(\mathcal L_\infty-\lambda)^{-1}w \|\leq \|(\mathcal L-\mathcal L_\infty)(\mathcal L_\infty-\lambda)^{-1}w \|
$$


$$
\int |(\mathcal L-\mathcal L_\infty)(\mathcal L_\infty-\lambda)^{-1}w |^2dx= 
$$


